Working on the list reversal example, Hoare Logic proof.

Ann_Com.thy
@@ -1,5 +1,5 @@
 theory Ann_Com
-imports BExp
+imports BExp Star
 begin
 
 type_synonym address = nat
@@ -17,15 +17,18 @@ datatype com =
   Wait "newstate \<Rightarrow> bool"              ("WAIT _ END")
 
 fun list :: "newstate \<Rightarrow> (nat list) \<Rightarrow> nat \<Rightarrow> bool" where 
-"list s [] i = (i = (0::nat))"|
-"list s (x#xs) i = (\<exists>j. ((mem s) i = x) \<and> ((mem s) (i + 1) = j) \<and> list s xs j)"
+"list s [] i = (i = 0)"|
+"list s (x#xs) i = ((mem s) i = x \<and> list s xs ((mem s) (i + 1)))"
 
+
+(*
 fun reach_step::"newstate \<Rightarrow> nat \<Rightarrow> nat \<Rightarrow> nat \<Rightarrow> bool" where
 "reach_step s 0 i j = (i = j)"|
 "reach_step s (Suc n) i j = (\<exists> k. ((mem s) (i + 1) = k) \<and> (reach_step s n k j))"
 
 definition reach::"newstate \<Rightarrow> address \<Rightarrow> nat \<Rightarrow> bool" where
   "reach s i j \<equiv> (\<exists>n \<ge> 0. reach_step s n i j)"
+*)
 
 datatype acom =
   ABasic assn "newstate \<Rightarrow> newstate"    ("{_} BASIC _ ")   |
